# Change of Basis: A Complete Walkthrough

## Setup

Consider a two-dimensional Hilbert space $\mathcal{H} = \mathbb{C}^2$ describing a spin-½ particle.

### Initial Basis: z-basis

We begin with the standard basis aligned with the z-axis:

$$\mathcal{B}_z = \{|↑_z\rangle, |↓_z\rangle\}$$

In matrix representation:

$$|↑_z\rangle = \begin{bmatrix} 1 \\ 0 \end{bmatrix}, \quad |↓_z\rangle = \begin{bmatrix} 0 \\ 1 \end{bmatrix}$$

This basis is orthonormal:

$$\langle ↑_z | ↑_z \rangle = 1, \quad \langle ↓_z | ↓_z \rangle = 1, \quad \langle ↑_z | ↓_z \rangle = 0$$

### Target Basis: x-basis

We want to transform to the basis aligned with the x-axis:

$$\mathcal{B}_x = \{|↑_x\rangle, |↓_x\rangle\}$$

where:

$$|↑_x\rangle = \frac{1}{\sqrt{2}}(|↑_z\rangle + |↓_z\rangle) = \frac{1}{\sqrt{2}}\begin{bmatrix} 1 \\ 1 \end{bmatrix}$$

$$|↓_x\rangle = \frac{1}{\sqrt{2}}(|↑_z\rangle - |↓_z\rangle) = \frac{1}{\sqrt{2}}\begin{bmatrix} 1 \\ -1 \end{bmatrix}$$

---

## Step 1: Construct the Unitary Transformation Matrix

The unitary matrix $U$ that transforms from the z-basis to the x-basis has columns consisting of the new basis vectors expressed in the old basis.

$$U = \begin{bmatrix} | & | \\ |↑_x\rangle & |↓_x\rangle \\ | & | \end{bmatrix}_{z\text{-basis}}$$

Substituting the expressions:

$$U = \begin{bmatrix} \frac{1}{\sqrt{2}} & \frac{1}{\sqrt{2}} \\ \frac{1}{\sqrt{2}} & -\frac{1}{\sqrt{2}} \end{bmatrix} = \frac{1}{\sqrt{2}}\begin{bmatrix} 1 & 1 \\ 1 & -1 \end{bmatrix}$$

This is the Hadamard matrix.

---

## Step 2: Verify Unitarity

A matrix is unitary if $U^\dagger U = I$, where $U^\dagger$ is the conjugate transpose.

**Compute $U^\dagger$:**

$$U^\dagger = \frac{1}{\sqrt{2}}\begin{bmatrix} 1 & 1 \\ 1 & -1 \end{bmatrix}^\dagger = \frac{1}{\sqrt{2}}\begin{bmatrix} 1 & 1 \\ 1 & -1 \end{bmatrix}$$

(The matrix is real and symmetric, so $U^\dagger = U^T = U$)

**Compute $U^\dagger U$:**

$$U^\dagger U = \frac{1}{\sqrt{2}}\begin{bmatrix} 1 & 1 \\ 1 & -1 \end{bmatrix} \cdot \frac{1}{\sqrt{2}}\begin{bmatrix} 1 & 1 \\ 1 & -1 \end{bmatrix}$$

$$= \frac{1}{2}\begin{bmatrix} 1 & 1 \\ 1 & -1 \end{bmatrix}\begin{bmatrix} 1 & 1 \\ 1 & -1 \end{bmatrix}$$

$$= \frac{1}{2}\begin{bmatrix} 1+1 & 1-1 \\ 1-1 & 1+1 \end{bmatrix} = \frac{1}{2}\begin{bmatrix} 2 & 0 \\ 0 & 2 \end{bmatrix} = \begin{bmatrix} 1 & 0 \\ 0 & 1 \end{bmatrix} = I$$

The transformation is unitary.

---

## Step 3: Transform a State Vector

Consider an arbitrary state in the z-basis:

$$|\psi\rangle_z = \alpha |↑_z\rangle + \beta |↓_z\rangle = \begin{bmatrix} \alpha \\ \beta \end{bmatrix}_z$$

where $|\alpha|^2 + |\beta|^2 = 1$ (normalization condition).

**Apply the transformation:**

$$|\psi\rangle_x = U^\dagger |\psi\rangle_z$$

(Note: We use $U^\dagger$ to transform state vectors from the old basis to the new basis)

$$|\psi\rangle_x = \frac{1}{\sqrt{2}}\begin{bmatrix} 1 & 1 \\ 1 & -1 \end{bmatrix}\begin{bmatrix} \alpha \\ \beta \end{bmatrix}$$

$$= \frac{1}{\sqrt{2}}\begin{bmatrix} \alpha + \beta \\ \alpha - \beta \end{bmatrix}_x$$

**Interpretation:** The state $|\psi\rangle_x$ has components:

$$|\psi\rangle_x = \frac{\alpha + \beta}{\sqrt{2}} |↑_x\rangle + \frac{\alpha - \beta}{\sqrt{2}} |↓_x\rangle$$

---

## Step 4: Verify Norm Preservation

The norm must be preserved under unitary transformation:

$$\langle \psi | \psi \rangle_z = \langle \psi | \psi \rangle_x$$

**In z-basis:**

$$\langle \psi | \psi \rangle_z = |\alpha|^2 + |\beta|^2$$

**In x-basis:**

$$\langle \psi | \psi \rangle_x = \left|\frac{\alpha + \beta}{\sqrt{2}}\right|^2 + \left|\frac{\alpha - \beta}{\sqrt{2}}\right|^2$$

$$= \frac{1}{2}[|\alpha + \beta|^2 + |\alpha - \beta|^2]$$

$$= \frac{1}{2}[(\alpha + \beta)(\alpha^* + \beta^*) + (\alpha - \beta)(\alpha^* - \beta^*)]$$

$$= \frac{1}{2}[|\alpha|^2 + \alpha\beta^* + \alpha^*\beta + |\beta|^2 + |\alpha|^2 - \alpha\beta^* - \alpha^*\beta + |\beta|^2]$$

$$= \frac{1}{2}[2|\alpha|^2 + 2|\beta|^2] = |\alpha|^2 + |\beta|^2$$

The norm is preserved.

---

## Step 5: Transform an Operator

Consider an observable represented by operator $A$ in the z-basis. To find its representation in the x-basis, we use:

$$A_x = U^\dagger A_z U$$

**Example:** The spin operator $\sigma_z$ in the z-basis:

$$\sigma_z = \begin{bmatrix} 1 & 0 \\ 0 & -1 \end{bmatrix}_z$$

**Transform to x-basis:**

$$\sigma_{z,x} = U^\dagger \sigma_z U$$

$$= \frac{1}{\sqrt{2}}\begin{bmatrix} 1 & 1 \\ 1 & -1 \end{bmatrix} \begin{bmatrix} 1 & 0 \\ 0 & -1 \end{bmatrix} \frac{1}{\sqrt{2}}\begin{bmatrix} 1 & 1 \\ 1 & -1 \end{bmatrix}$$

**First multiply $\sigma_z U$:**

$$\begin{bmatrix} 1 & 0 \\ 0 & -1 \end{bmatrix} \frac{1}{\sqrt{2}}\begin{bmatrix} 1 & 1 \\ 1 & -1 \end{bmatrix} = \frac{1}{\sqrt{2}}\begin{bmatrix} 1 & 1 \\ -1 & 1 \end{bmatrix}$$

**Then multiply $U^\dagger (\sigma_z U)$:**

$$\frac{1}{\sqrt{2}}\begin{bmatrix} 1 & 1 \\ 1 & -1 \end{bmatrix} \frac{1}{\sqrt{2}}\begin{bmatrix} 1 & 1 \\ -1 & 1 \end{bmatrix}$$

$$= \frac{1}{2}\begin{bmatrix} 1-1 & 1+1 \\ 1+1 & 1-1 \end{bmatrix} = \frac{1}{2}\begin{bmatrix} 0 & 2 \\ 2 & 0 \end{bmatrix} = \begin{bmatrix} 0 & 1 \\ 1 & 0 \end{bmatrix}_x$$

This is $\sigma_x$ in the x-basis, as expected.

---

## Step 6: Verify Eigenvalue Preservation

The eigenvalues of an operator are basis-independent.

**Eigenvalues of $\sigma_z$ in z-basis:**

$$\det(\sigma_z - \lambda I) = \det\begin{bmatrix} 1-\lambda & 0 \\ 0 & -1-\lambda \end{bmatrix} = (1-\lambda)(-1-\lambda) = 0$$

$$\lambda_1 = 1, \quad \lambda_2 = -1$$

**Eigenvalues of $\sigma_{z,x}$ in x-basis:**

$$\det(\sigma_{z,x} - \lambda I) = \det\begin{bmatrix} -\lambda & 1 \\ 1 & -\lambda \end{bmatrix} = \lambda^2 - 1 = 0$$

$$\lambda_1 = 1, \quad \lambda_2 = -1$$

The eigenvalues are identical, confirming they are basis-independent physical observables.

---

## Summary

The change of basis procedure:

1. **Construct $U$:** Columns are new basis vectors in old basis representation
2. **Verify unitarity:** Check $U^\dagger U = I$
3. **Transform states:** $|\psi\rangle_{\text{new}} = U^\dagger |\psi\rangle_{\text{old}}$
4. **Verify norm preservation:** $\langle \psi | \psi \rangle$ unchanged
5. **Transform operators:** $A_{\text{new}} = U^\dagger A_{\text{old}} U$
6. **Verify eigenvalue preservation:** Spectrum is basis-independent

The physical content (probabilities, measurement outcomes) remains invariant under unitary transformations.